lib/bv32_ops.dfy
@@ -1,4 +1,6 @@
 include "generic_bv_ops.dfy"
+include "DivModNeg.dfy"
+include "../std_lib/src/NonlinearArithmetic/Power2.dfy"
 
 module bv32_seq refines LittleEndianNat
 {
@@ -12,7 +14,9 @@ module bv32_seq refines LittleEndianNat
 
 module bv32_ops refines generic_bv_ops
 {
-    import opened BVSEQ = bv32_seq 
+    import opened BVSEQ = bv32_seq
+    import DivModNeg
+    import Power2
 
     // half word base
     function method HW_BASE(): nat
@@ -64,4 +68,92 @@ module bv32_ops refines generic_bv_ops
     {
         if ((x as bv256 >> 32) & 1 == 1) then 1 else 0
     }
+
+    function uint32_lt(x: uint, y: uint): uint
+    {
+        if x < y then 1 else 0
+    }
+
+    function uint32_le(x: uint, y: uint): uint
+    {
+      if x <= y then 1 else 0
+    }
+
+    // function method uint32_full_mul(x: uint, y: uint): (r: nat)
+    //     ensures r == x * y
+    //     ensures r < DW_BASE()
+    // {
+    //     x * y
+    // }
+
+    function method uint32_mul(x: uint, y: uint): uint
+    {
+        full_mul_bound_lemma(x, y);
+        dw_lh(x * y)
+    }
+
+    function method uint32_mulhu(x: uint, y: uint): uint
+    {
+        full_mul_bound_lemma(x, y);
+        dw_uh(x * y)
+    }
+
+    function method uint32_add(x: uint, y: uint): uint
+    {
+        add(x, y)
+    }
+
+    function method to_uint32(x: sint): uint
+    {
+        to_2s_comp(x)
+    }
+
+    function method to_int32(x: uint): sint
+    {
+        if x < integers.BASE_31 then x else x - integers.BASE_32
+    }
+
+    lemma signed_conversion_lemma(x: sint)
+        ensures to_int32(to_uint32(x)) == x
+    {
+    }
+
+    function method int32_rs(x: sint, shift: nat) : sint
+    {
+        DivModNeg.LemmaDivBounded(x, Power2.Pow2(shift));
+        x / Power2.Pow2(shift)
+    }
+
+    function method uint32_ls(x: uint, amount: uint) : (r: uint)
+        requires amount < 32;
+    {
+        ls(x, amount)
+    }
+
+    function method uint32_xor(x: uint, y: uint): uint
+    {
+        xor(x, y)
+    }
+
+    function method uint32_or(x: uint, y: uint): uint
+    {
+        or(x, y)
+    }
+
+    function method uint32_and(x: uint, y: uint): uint
+    {
+        and(x, y)
+    }
+
+    function method uint32_rs(x: uint, amount: uint): uint
+        requires amount < 32;
+    {
+        rs(x, amount)
+    }
+
+    function method uint32_sub(x: uint, y: uint): uint
+    {
+        sub(x, y)
+    }
 }
+        
