lib/generic_mm_lemmas.dfy
@@ -1,7 +1,4 @@
 include "generic_bv_ops.dfy"
-include "bv256_ops.dfy"
-include "../arch/otbn/abstraction.i.dfy"
-include "mul256_nl_lemma.i.dfy"
 
 abstract module generic_mm_lemmas {
     import opened GBV: generic_bv_ops
@@ -93,22 +90,27 @@ abstract module generic_mm_lemmas {
         to_nat([x_lh, x_uh]) + to_nat([y_lh, y_uh]) < DW_BASE()
     }
 
+    function add_carry_bit(x: uint, y: uint): uint1
+    {
+        if x + y >= BASE() then 1 else 0
+    }
+
     lemma dw_add_lemma(
         x_lh: uint, x_uh: uint,
         y_lh: uint, y_uh: uint,
-        c1: uint1, c2: uint1,
-        z_lh: uint, z_uh: uint)
+        carry: uint1)
     returns (z: dw_view_t)
-
         requires dw_add_is_safe(x_lh, x_uh, y_lh, y_uh);
-        requires (z_lh, c1) == GBV.addc(x_lh, y_lh, 0);
-        requires (z_uh, c2) == GBV.addc(x_uh, y_uh, c1);
-        
-        ensures z.full == to_nat([z_lh, z_uh]) == to_nat([x_lh, x_uh]) + to_nat([y_lh, y_uh]);
-        ensures z.lh ==  z_lh;
-        ensures z.uh ==  z_uh;
+        requires carry == add_carry_bit(x_lh, y_lh);
+        ensures (z.lh, carry) == GBV.addc(x_lh, y_lh, 0);
+        ensures (z.uh, 0) == GBV.addc(x_uh, y_uh, carry);
+        ensures z.full == to_nat([x_lh, x_uh]) + to_nat([y_lh, y_uh]);
         ensures y_uh == 0 ==> z.full == to_nat([x_lh, x_uh]) + y_lh;
     {
+        var (z_lh, c1) := GBV.addc(x_lh, y_lh, 0);
+        var (z_uh, c2) := GBV.addc(x_uh, y_uh, c1);
+        assert c1 == carry;
+
         var x_full := to_nat([x_lh, x_uh]);
         var y_full := to_nat([y_lh, y_uh]);
         var z_full := to_nat([z_lh, z_uh]);
@@ -154,15 +156,53 @@ abstract module generic_mm_lemmas {
         }
 
         z := dw_view_cons(z_lh, z_uh, full);
+        // assert (z.lh, c1) == GBV.addc(x_lh, y_lh, 0);
     }
 
-    // method dw_add(x_lh: uint, x_uh: uint, y_lh: uint, y_uh: uint)
-    //     requires dw_add_is_safe(x_lh, x_uh, y_lh, y_uh);
-    // {
-    //     var (z_lh, c1) := GBV.addc(x_lh, y_lh, 0);
-    //     var (z_uh, c2) := GBV.addc(x_uh, y_uh, c1);
-    //     dw_add_lemma(x_lh, x_uh, y_lh, y_uh, c1, c2, z_lh, z_uh);
-    // }
+    lemma mul_add_lemma(
+        xs: seq<uint>, ys: seq<uint>, 
+        carry: uint1, a: uint, b: uint)
+    returns (z: dw_view_t)
+        requires |xs| == |ys| == 2;
+        requires to_nat(xs) == a * b;
+        requires ys[1] == 0;
+        requires carry == add_carry_bit(xs[0], ys[0]);
+        ensures (z.lh, carry) == GBV.addc(xs[0], ys[0], 0);
+        ensures (z.uh, 0) == GBV.addc(xs[1], ys[1], carry);
+        ensures z.full == to_nat(xs) + ys[0];
+    {
+        assert xs == [xs[0], xs[1]];
+        mul_add_bound_lemma(a, b, ys[0]);
+        var y_val := to_nat([ys[0], ys[1]]);
+        assert y_val == ys[0] by {
+            GBV.BVSEQ.LemmaSeqLen2([ys[0], ys[1]]);
+            assert y_val == ys[0] + 0 * BASE();
+        }
+        assert to_nat([xs[0], xs[1]]) + y_val < DW_BASE();
+        z := dw_add_lemma(xs[0], xs[1], ys[0], ys[1], carry);
+    }
+
+    lemma mul_double_add_lemma(
+        xs: seq<uint>, ys: seq<uint>, carry: uint1, a: uint, b: uint, c: uint)
+    returns (z: dw_view_t)
+        requires |xs| == |ys| == 2;
+        requires to_nat(xs) == a * b + c;
+        requires ys[1] == 0;
+        requires carry == add_carry_bit(xs[0], ys[0]);
+        ensures (z.lh, carry) == GBV.addc(xs[0], ys[0], 0);
+        ensures (z.uh, 0) == GBV.addc(xs[1], ys[1], carry);
+        ensures z.full == to_nat(xs) + ys[0];
+    {
+        mul_double_add_bound_lemma(a, b, c, ys[0]);
+        assert xs == [xs[0], xs[1]];
+        var y_val := to_nat([ys[0], ys[1]]);
+        assert y_val == ys[0] by {
+            GBV.BVSEQ.LemmaSeqLen2([ys[0], ys[1]]);
+            assert y_val == ys[0] + 0 * BASE();
+        }
+        assert to_nat([xs[0], xs[1]]) +y_val < DW_BASE();
+        z := dw_add_lemma(xs[0], xs[1], ys[0], ys[1], carry);
+    }
 
 /* end section on double word addtion */
 
@@ -1014,265 +1054,4 @@ abstract module generic_mm_lemmas {
     }
 
 /* end section on mont mod exp */
-
 }
-
-module bv256_mm_lemmas refines generic_mm_lemmas {
-    import opened GBV = bv256_ops
-    import opened ot_machine
-    import opened ot_abstraction
-    import opened mul256_nl_lemma
-
-    type uint512_view_t = dw_view_t
-
-    predicate valid_uint512_view(
-        wdrs: wdrs_t, num: uint512_view_t,
-        li: int, ui: int)
-        requires -1 <= li < BASE_5;
-        requires -1 <= ui < BASE_5;
-    {
-        && (li == NA || wdrs[li] == num.lh)
-        && (ui == NA || wdrs[ui] == num.uh)
-    }
-
-    const NUM_WORDS := 12
-
-    datatype mvars = mvars(
-        x_it: iter_t,
-        y_it: iter_t,
-
-        m_it: iter_t,
-        m0d_it: iter_t,
-        rr_it: iter_t,
-        sig_it: iter_t,
-        rsa: rsa_params)
-
-    predicate mvars_iter_init(iter: iter_t, heap: heap_t, address: int, value: int)
-    {
-        && (address >= 0 ==> iter_inv(iter, heap, address))
-        && (value >= 0 ==> to_nat(iter.buff) == value)
-        && iter.index == 0
-        && |iter.buff| == NUM_WORDS
-    }
-
-    predicate m0d_it_inv(iter: iter_t, heap: heap_t, address: int)
-    {
-        && (address >= 0 ==> iter_inv(iter, heap, address))
-        && iter.index == 0
-        && |iter.buff| == 1
-    }
-
-    predicate mvars_inv(
-        vars: mvars,
-        heap: heap_t,
-        x_ptr: int,
-        y_ptr: int,
-        m_ptr: int,
-        m0d_ptr: int,
-        rr_ptr: int,
-        sig_ptr: int)
-    {
-        && rsa_params_inv(vars.rsa)
-
-        && mvars_iter_init(vars.x_it, heap, x_ptr, NA)
-        && mvars_iter_init(vars.y_it, heap, y_ptr, NA)
-        && mvars_iter_init(vars.sig_it, heap, sig_ptr, vars.rsa.SIG)
-        && mvars_iter_init(vars.m_it, heap, m_ptr, vars.rsa.M)
-        && mvars_iter_init(vars.rr_it, heap, rr_ptr, vars.rsa.RR)
-
-        && m0d_it_inv(vars.m0d_it, heap, m0d_ptr)
-        && vars.m0d_it.buff[0] == vars.rsa.M0D
-    }
-
-    predicate mvars_init(
-        vars: mvars,
-        heap: heap_t,
-        m_ptr: uint32,
-        m0d_ptr: uint32,
-        rr_ptr: uint32,
-        sig_ptr: uint32,
-        out_ptr: uint32)
-    {
-        && rsa_params_inv(vars.rsa)
-        && vars.rsa.E0 < BASE_32
-        && is_xword_pointee(heap, 0, vars.rsa.E0)
-        && is_xword_pointee(heap, 4, NUM_WORDS)
-        && is_xword_pointee(heap, 16, m_ptr)
-        && is_xword_pointee(heap, 8, m0d_ptr)
-        && is_xword_pointee(heap, 12, rr_ptr)
-        && is_xword_pointee(heap, 20, sig_ptr)
-        && is_xword_pointee(heap, 28, out_ptr)
-
-        && mvars_inv(vars, heap, NA, NA, m_ptr, m0d_ptr, rr_ptr, sig_ptr)
-        && buff_base_ptr_valid(heap, out_ptr)
-        && |heap[out_ptr].b| == NUM_WORDS
-
-        && out_ptr != m0d_ptr
-        && out_ptr != rr_ptr
-        && out_ptr != m_ptr
-        && out_ptr != sig_ptr
-    }
-
-    lemma mont_word_mul_add_bound_lemma_0(
-        xs: seq<uint256>, ys: seq<uint256>, a: uint256, b: uint256)
-        requires |xs| == |ys| == 2;
-        requires to_nat(xs) == a * b;
-        requires ys[1] == 0;
-        ensures dw_add_is_safe(xs[0], xs[1], ys[0], ys[1]);
-    {
-        mul_add_bound_lemma(a, b, ys[0]);
-        assert xs == [xs[0], xs[1]];
-        assert to_nat([ys[0], ys[1]]) == ys[0] by {
-            GBV.BVSEQ.LemmaSeqLen2([ys[0], ys[1]]);
-        }
-        assert to_nat([xs[0], xs[1]]) + to_nat([ys[0], ys[1]]) < DW_BASE();
-    }
-
-    lemma mont_word_mul_add_bound_lemma_1(
-        xs: seq<uint256>, ys: seq<uint256>, a: uint256, b: uint256, c: uint256)
-        requires |xs| == |ys| == 2;
-        requires to_nat(xs) == a * b + c;
-        requires ys[1] == 0;
-        ensures dw_add_is_safe(xs[0], xs[1], ys[0], ys[1]);
-    {
-        mul_double_add_bound_lemma(a, b, c, ys[0]);
-        assert xs == [xs[0], xs[1]];
-        assert to_nat([ys[0], ys[1]]) == ys[0] by {
-            GBV.BVSEQ.LemmaSeqLen2([ys[0], ys[1]]);
-        }
-        assert to_nat([xs[0], xs[1]]) + to_nat([ys[0], ys[1]]) < DW_BASE();
-    }
-
-    lemma mul256_correct_lemma(
-        p0: uint256,
-        p1: uint256,
-        p2: uint256,
-        p3: uint256,
-        p4: uint256,
-        p5: uint256,
-        p6: uint256,
-        p7: uint256,
-        p8: uint256,
-        p9: uint256,
-        p10: uint256,
-        p11: uint256,
-        p12: uint256,
-        p13: uint256,
-        p14: uint256,
-        p15: uint256,
-        r0: uint256,
-        r1: uint256,
-        r2: uint256,
-        r3: uint256,
-
-        x: uint256,
-        y: uint256,
-
-        t0: uint256,
-        t1: uint256,
-        t2: uint256,
-        u0: uint256,
-        u1: uint256,
-        u2: uint256,
-        wacc: uint256)
-
-        requires
-            && p0 == otbn_qmul(x, 0, y, 0)
-            && p1 == otbn_qmul(x, 1, y, 0)
-            && p2 == otbn_qmul(x, 0, y, 1)
-            && p3 == otbn_qmul(x, 2, y, 0)
-            && p4 == otbn_qmul(x, 1, y, 1)
-            && p5 == otbn_qmul(x, 0, y, 2)
-            && p6 == otbn_qmul(x, 3, y, 0)
-            && p7 == otbn_qmul(x, 2, y, 1)
-            && p8 == otbn_qmul(x, 1, y, 2)
-            && p9 == otbn_qmul(x, 0, y, 3)
-            && p10 == otbn_qmul(x, 3, y, 1)
-            && p11 == otbn_qmul(x, 2, y, 2)
-            && p12 == otbn_qmul(x, 1, y, 3)
-            && p13 == otbn_qmul(x, 3, y, 2)
-            && p14 == otbn_qmul(x, 2, y, 3)
-            && p15 == otbn_qmul(x, 3, y, 3)
-            && r0 == p0 + (p1 + p2) * B
-            && r1 == uh(r0) + p3 + p4 + p5 + (p6 + p7 + p8 + p9) * B
-            && r2 == uh(r1) + p10 + p11 + p12 + (p13 + p14) * B
-            && r3 == uh(r2) + p15
-            && t1 == otbn_hwb(t0, lh(r0), true)
-            && t2 == otbn_hwb(t1, lh(r1), false)
-            && u1 == otbn_hwb(u0, lh(r2), true)
-            && u2 == otbn_hwb(u1, lh(r3), false)
-            && wacc == uh(r3)
-
-        ensures
-            to_nat([t2, u2]) == x * y;
-    {
-        assert t2 == lh(r0) + lh(r1) * B2 by {
-            otbn_hwb_lemma(t0, t1, t2, lh(r0), lh(r1));
-        }
-
-        assert u2 == lh(r2) + lh(r3) * B2 by {
-            otbn_hwb_lemma(u0, u1, u2, lh(r2), lh(r3));
-        }
-
-        var x_0, x_1, x_2, x_3  := otbn_qsel(x, 0), otbn_qsel(x, 1), otbn_qsel(x, 2), otbn_qsel(x, 3);
-
-        assert x == x_0 + x_1 * B + x_2 * B2 + x_3 * B3 by {
-            uint256_quarter_split_lemma(x);
-        }
-
-        var y_0, y_1, y_2, y_3  := otbn_qsel(y, 0), otbn_qsel(y, 1), otbn_qsel(y, 2), otbn_qsel(y, 3);
-
-        assert y == y_0 + y_1 * B + y_2 * B2 + y_3 * B3 by {
-            uint256_quarter_split_lemma(y);
-        }
-
-        calc {
-            t2 + u2 * B4 + wacc * B8;
-                { half_split_lemma(r3); }
-            t2 + (lh(r2) + r3 * B2) * B4;
-                { half_split_lemma(r2); }
-            t2 + (r2 - uh(r2) * B2 + r3 * B2) * B4;
-            t2 + r2 * B4 - uh(r2) * B2 * B4 + r3 * B2 * B4;
-            lh(r0) + lh(r1) * B2 + r2 * B4 - uh(r2) * B2 * B4 + r3 * B2 * B4;
-                { LemmaMulIsAssociativeAuto(); }
-            lh(r0) + lh(r1) * B2 + r2 * B4 + (r3 - uh(r2)) * B6;
-            lh(r0) + lh(r1) * B2 + r2 * B4 + p15 * B6;
-                { half_split_lemma(r1); }
-            lh(r0) + (r1 - uh(r1) * B2) * B2 + r2 * B4 + p15 * B6;
-            lh(r0) + r1 * B2 - uh(r1) * B4 + r2 * B4 + p15 * B6;
-            lh(r0) + r1 * B2 + (r2 - uh(r1)) * B4 + p15 * B6;
-            lh(r0) + r1 * B2 + (p10 + p11 + p12 + (p13 + p14) * B) * B4 + p15 * B6;
-            lh(r0) + r1 * B2 + ((p10 + p11 + p12) + (p13 + p14) * B) * B4 + p15 * B6;
-                { LemmaMulIsDistributiveAddOtherWayAuto(); }
-            lh(r0) + r1 * B2 + (p10 + p11 + p12) * B4 + ((p13 + p14) * B) * B4 + p15 * B6;
-                { LemmaMulIsCommutativeAuto(); }
-            lh(r0) + r1 * B2 + (p10 + p11 + p12) * B4 + (p13 + p14) * B5 + p15 * B6;
-                { half_split_lemma(r0); }
-            p0 + (p1 + p2) * B + (p3 + p4 + p5) * B2 + (p6 + p7 + p8 + p9) * B3 + (p10 + p11 + p12) * B4 + (p13 + p14) * B5 + p15 * B6;
-                {
-                    reveal otbn_qmul();
-                    mul256_canonize_lemma(
-                        p0, p1, p2, p3,
-                        p4, p5, p6, p7,
-                        p8, p9, p10, p11,
-                        p12, p13, p14, p15,
-                        x, x_0, x_1, x_2, x_3,
-                        y, y_0, y_1,y_2, y_3);
-                }
-            x * y;
-        }
-
-        assert wacc == 0 by {
-            assert x * y <= (B4 - 1) * (B4 - 1) by {
-                Mul.LemmaMulUpperBoundAuto();
-            }
-            assert x * y <= B8;
-        }
-
-        assert to_nat([t2, u2]) == x * y by {
-            GBV.BVSEQ.LemmaSeqLen2([t2, u2]);
-        }
-    }
-
-}
-
