lib/bv256_mm_lemmas.s.dfy
@@ -1,0 +1,213 @@
+include "../arch/otbn/abstraction.i.dfy"
+include "bv256_ops.dfy"
+include "generic_mm_lemmas.dfy"
+include "mul256_nl_lemma.i.dfy"
+
+module bv256_mm_lemmas refines generic_mm_lemmas {
+    import opened GBV = bv256_ops
+    import opened ot_machine
+    import opened ot_abstraction
+    import opened mul256_nl_lemma
+
+    type uint512_view_t = dw_view_t
+
+    predicate valid_uint512_view(
+        wdrs: wdrs_t, num: uint512_view_t,
+        li: int, ui: int)
+        requires -1 <= li < BASE_5;
+        requires -1 <= ui < BASE_5;
+    {
+        && (li == NA || wdrs[li] == num.lh)
+        && (ui == NA || wdrs[ui] == num.uh)
+    }
+
+    const NUM_WORDS := 12
+
+    datatype mvars = mvars(
+        x_it: iter_t,
+        y_it: iter_t,
+
+        m_it: iter_t,
+        m0d_it: iter_t,
+        rr_it: iter_t,
+        sig_it: iter_t,
+        rsa: rsa_params)
+
+    predicate mvars_iter_init(iter: iter_t, heap: heap_t, address: int, value: int)
+    {
+        && (address >= 0 ==> iter_inv(iter, heap, address))
+        && (value >= 0 ==> to_nat(iter.buff) == value)
+        && iter.index == 0
+        && |iter.buff| == NUM_WORDS
+    }
+
+    predicate m0d_it_inv(iter: iter_t, heap: heap_t, address: int)
+    {
+        && (address >= 0 ==> iter_inv(iter, heap, address))
+        && iter.index == 0
+        && |iter.buff| == 1
+    }
+
+    predicate mvars_inv(
+        vars: mvars,
+        heap: heap_t,
+        x_ptr: int,
+        y_ptr: int,
+        m_ptr: int,
+        m0d_ptr: int,
+        rr_ptr: int,
+        sig_ptr: int)
+    {
+        && rsa_params_inv(vars.rsa)
+
+        && mvars_iter_init(vars.x_it, heap, x_ptr, NA)
+        && mvars_iter_init(vars.y_it, heap, y_ptr, NA)
+        && mvars_iter_init(vars.sig_it, heap, sig_ptr, vars.rsa.SIG)
+        && mvars_iter_init(vars.m_it, heap, m_ptr, vars.rsa.M)
+        && mvars_iter_init(vars.rr_it, heap, rr_ptr, vars.rsa.RR)
+
+        && m0d_it_inv(vars.m0d_it, heap, m0d_ptr)
+        && vars.m0d_it.buff[0] == vars.rsa.M0D
+    }
+
+    predicate mvars_init(
+        vars: mvars,
+        heap: heap_t,
+        m_ptr: uint32,
+        m0d_ptr: uint32,
+        rr_ptr: uint32,
+        sig_ptr: uint32,
+        out_ptr: uint32)
+    {
+        && rsa_params_inv(vars.rsa)
+        && vars.rsa.E0 < BASE_32
+        && is_xword_pointee(heap, 0, vars.rsa.E0)
+        && is_xword_pointee(heap, 4, NUM_WORDS)
+        && is_xword_pointee(heap, 16, m_ptr)
+        && is_xword_pointee(heap, 8, m0d_ptr)
+        && is_xword_pointee(heap, 12, rr_ptr)
+        && is_xword_pointee(heap, 20, sig_ptr)
+        && is_xword_pointee(heap, 28, out_ptr)
+
+        && mvars_inv(vars, heap, NA, NA, m_ptr, m0d_ptr, rr_ptr, sig_ptr)
+        && buff_base_ptr_valid(heap, out_ptr)
+        && |heap[out_ptr].b| == NUM_WORDS
+
+        && out_ptr != m0d_ptr
+        && out_ptr != rr_ptr
+        && out_ptr != m_ptr
+        && out_ptr != sig_ptr
+    }
+
+  
+
+    lemma mul256_correct_lemma(
+        p0: uint256, p1: uint256, p2: uint256, p3: uint256,
+        p4: uint256, p5: uint256, p6: uint256, p7: uint256,
+        p8: uint256, p9: uint256, p10: uint256, p11: uint256,
+        p12: uint256, p13: uint256, p14: uint256, p15: uint256,
+        r0: uint256, r1: uint256, r2: uint256, r3: uint256,
+        x: uint256, y: uint256,
+        t0: uint256, t1: uint256, t2: uint256,
+        u0: uint256, u1: uint256, u2: uint256,
+        wacc: uint256)
+
+        requires
+            && p0 == otbn_qmul(x, 0, y, 0)
+            && p1 == otbn_qmul(x, 1, y, 0)
+            && p2 == otbn_qmul(x, 0, y, 1)
+            && p3 == otbn_qmul(x, 2, y, 0)
+            && p4 == otbn_qmul(x, 1, y, 1)
+            && p5 == otbn_qmul(x, 0, y, 2)
+            && p6 == otbn_qmul(x, 3, y, 0)
+            && p7 == otbn_qmul(x, 2, y, 1)
+            && p8 == otbn_qmul(x, 1, y, 2)
+            && p9 == otbn_qmul(x, 0, y, 3)
+            && p10 == otbn_qmul(x, 3, y, 1)
+            && p11 == otbn_qmul(x, 2, y, 2)
+            && p12 == otbn_qmul(x, 1, y, 3)
+            && p13 == otbn_qmul(x, 3, y, 2)
+            && p14 == otbn_qmul(x, 2, y, 3)
+            && p15 == otbn_qmul(x, 3, y, 3)
+            && r0 == p0 + (p1 + p2) * B
+            && r1 == uh(r0) + p3 + p4 + p5 + (p6 + p7 + p8 + p9) * B
+            && r2 == uh(r1) + p10 + p11 + p12 + (p13 + p14) * B
+            && r3 == uh(r2) + p15
+            && t1 == otbn_hwb(t0, lh(r0), true)
+            && t2 == otbn_hwb(t1, lh(r1), false)
+            && u1 == otbn_hwb(u0, lh(r2), true)
+            && u2 == otbn_hwb(u1, lh(r3), false)
+            && wacc == uh(r3)
+
+        ensures
+            to_nat([t2, u2]) == x * y;
+    {
+        assert t2 == lh(r0) + lh(r1) * B2 by {
+            otbn_hwb_lemma(t0, t1, t2, lh(r0), lh(r1));
+        }
+
+        assert u2 == lh(r2) + lh(r3) * B2 by {
+            otbn_hwb_lemma(u0, u1, u2, lh(r2), lh(r3));
+        }
+
+        var x_0, x_1, x_2, x_3  := otbn_qsel(x, 0), otbn_qsel(x, 1), otbn_qsel(x, 2), otbn_qsel(x, 3);
+
+        assert x == x_0 + x_1 * B + x_2 * B2 + x_3 * B3 by {
+            uint256_quarter_split_lemma(x);
+        }
+
+        var y_0, y_1, y_2, y_3  := otbn_qsel(y, 0), otbn_qsel(y, 1), otbn_qsel(y, 2), otbn_qsel(y, 3);
+
+        assert y == y_0 + y_1 * B + y_2 * B2 + y_3 * B3 by {
+            uint256_quarter_split_lemma(y);
+        }
+
+        calc {
+            t2 + u2 * B4 + wacc * B8;
+                { half_split_lemma(r3); }
+            t2 + (lh(r2) + r3 * B2) * B4;
+                { half_split_lemma(r2); }
+            t2 + (r2 - uh(r2) * B2 + r3 * B2) * B4;
+            t2 + r2 * B4 - uh(r2) * B2 * B4 + r3 * B2 * B4;
+            lh(r0) + lh(r1) * B2 + r2 * B4 - uh(r2) * B2 * B4 + r3 * B2 * B4;
+                { LemmaMulIsAssociativeAuto(); }
+            lh(r0) + lh(r1) * B2 + r2 * B4 + (r3 - uh(r2)) * B6;
+            lh(r0) + lh(r1) * B2 + r2 * B4 + p15 * B6;
+                { half_split_lemma(r1); }
+            lh(r0) + (r1 - uh(r1) * B2) * B2 + r2 * B4 + p15 * B6;
+            lh(r0) + r1 * B2 - uh(r1) * B4 + r2 * B4 + p15 * B6;
+            lh(r0) + r1 * B2 + (r2 - uh(r1)) * B4 + p15 * B6;
+            lh(r0) + r1 * B2 + (p10 + p11 + p12 + (p13 + p14) * B) * B4 + p15 * B6;
+            lh(r0) + r1 * B2 + ((p10 + p11 + p12) + (p13 + p14) * B) * B4 + p15 * B6;
+                { LemmaMulIsDistributiveAddOtherWayAuto(); }
+            lh(r0) + r1 * B2 + (p10 + p11 + p12) * B4 + ((p13 + p14) * B) * B4 + p15 * B6;
+                { LemmaMulIsCommutativeAuto(); }
+            lh(r0) + r1 * B2 + (p10 + p11 + p12) * B4 + (p13 + p14) * B5 + p15 * B6;
+                { half_split_lemma(r0); }
+            p0 + (p1 + p2) * B + (p3 + p4 + p5) * B2 + (p6 + p7 + p8 + p9) * B3 + (p10 + p11 + p12) * B4 + (p13 + p14) * B5 + p15 * B6;
+                {
+                    reveal otbn_qmul();
+                    mul256_canonize_lemma(
+                        p0, p1, p2, p3,
+                        p4, p5, p6, p7,
+                        p8, p9, p10, p11,
+                        p12, p13, p14, p15,
+                        x, x_0, x_1, x_2, x_3,
+                        y, y_0, y_1,y_2, y_3);
+                }
+            x * y;
+        }
+
+        assert wacc == 0 by {
+            assert x * y <= (B4 - 1) * (B4 - 1) by {
+                Mul.LemmaMulUpperBoundAuto();
+            }
+            assert x * y <= B8;
+        }
+
+        assert to_nat([t2, u2]) == x * y by {
+            GBV.BVSEQ.LemmaSeqLen2([t2, u2]);
+        }
+    }
+}
+
