lib/bv32_mm_lemmas.i.dfy
@@ -1,0 +1,33 @@
+include "../arch/riscv/machine.s.dfy"
+include "generic_mm_lemmas.dfy"
+include "bv32_ops.dfy"
+
+module bv32_mm_lemmas refines generic_mm_lemmas {
+    import opened GBV = bv32_ops
+
+    type uint64_view_t = dw_view_t
+
+    predicate valid_uint64_view(
+        num: uint64_view_t,
+        lh: uint32, uh: uint32)
+    {
+        && lh == num.lh
+        && uh == num.uh
+    }
+
+    lemma mul32_correct_lemma(a: uint32, b: uint32, c: uint32, d: uint32)
+        requires c == uint32_mul(a, b);
+        requires d == uint32_mulhu(a, b);
+        ensures to_nat([c, d]) == a * b;
+    {
+        reveal dw_lh();
+        reveal dw_uh();
+
+        var full := a * b;
+        dw_split_lemma(full);
+
+        GBV.BVSEQ.LemmaSeqLen2([c, d]);
+    }
+
+
+}
